\documentclass{article}
\usepackage{epsfig}
\pagestyle{empty}
\begin{document}
$\sigma \ge 0$
\pagebreak

$\phi$
\pagebreak

$ \left(p_1 \dots p_N \right)$
\pagebreak

$m$
\pagebreak

$ \left( p_{i_1} \dots p_{i_m} \right), i_1 < i_2 < \dots < i_m, m \le N, i_j \le N$
\pagebreak

$ \left(v^0_1 \dots v^0_N \right)$
\pagebreak

\[ \mathbb{R}^{N \times 1} \mapsto \mathbb{R}^{m \times 1} : \left( \begin{array}{c} v_1^0 \\ \vdots \\ v_N^0 \end{array} \right) \mapsto \left( \begin{array}{c} v_{i_1}^0 \\ \vdots \\ v_{i_m}^0 \end{array} \right) \]
\pagebreak

\[ \vec{r} = \left( \begin{array}{c} r_{i_1} \\ \vdots \\ r_{i_m} \end{array} \right) = \left( \begin{array}{c} v_{i_1} \\ \vdots \\ v_{i_m} \end{array} \right) - \mathrm{Proj} \left( \begin{array}{c} v^0_{1} \\ \vdots \\ v^0_{N} \end{array} \right) = \vec{v} - \mathrm{Proj} \left( \vec{v}^0 \right) \]
\pagebreak

$\mathrm{Proj}$
\pagebreak

$\vec{v}$
\pagebreak

$\vec{v}^0$
\pagebreak

\[ \vec{r} = \left( \begin{array}{c} r_{i_1} \\ \vdots \\ r_{i_m} \end{array} \right) = \left( \begin{array}{c} v_{i_1} \\ \vdots \\ v_{i_m} \end{array} \right) - \left( \begin{array}{c} v^0_{1} \\ \vdots \\ v^0_{N} \end{array} \right) = \vec{v} - \left( \vec{v}^0 \right) \]
\pagebreak

$ xy $
\pagebreak

$ z $
\pagebreak

$ yz $
\pagebreak

$ x $
\pagebreak

$ zx $
\pagebreak

$ y $
\pagebreak

$ r_{inner}=0 $
\pagebreak

$ z$
\pagebreak

$ r_{inner}>0 $
\pagebreak

$ r = r_{outer} $
\pagebreak

$ r = r_{inner} $
\pagebreak

$ r_{inner}>0$
\pagebreak

$ \phi < \pi $
\pagebreak

$z$
\pagebreak

$ r = r_{outer}$
\pagebreak

$ \phi $
\pagebreak

$x$
\pagebreak

$ x$
\pagebreak

$y$
\pagebreak

$ \tan(\alpha) $
\pagebreak

$ z_min $
\pagebreak

$ z_max $
\pagebreak

$x^2 + y^2 = z^2 \tan \alpha$
\pagebreak

$\alpha$
\pagebreak

$t$
\pagebreak

$x_1$
\pagebreak

$x_2$
\pagebreak

$(x,y,z) = \vec x_1 + (\vec x_2 - \vec x_2) t $
\pagebreak

$(x,y,z)$
\pagebreak

$ \vec x_d = \frac{\vec x_2 - \vec x_1}{|\vec x_2 - \vec x_1|} $
\pagebreak

$t^2 (x_d^2 + y_d^2 - z_d^2 \tan^2 \alpha) + 2 t (x_1 x_d + y_1 y_d - z_1 z_d \tan^2 \alpha) + (x_1^2 + y_1^2 - z_1^2 \tan^2 \alpha) = 0 $
\pagebreak

$x_d$
\pagebreak

$ 2\cdot\phi_{half}$
\pagebreak

$ \phi_{ave} $
\pagebreak

$ d_0 $
\pagebreak

$ \vec d = \vec m - \vec c $
\pagebreak

$ \vec d $
\pagebreak

$ \vec{measY}= \vec{Acts::eLOC_Z} $
\pagebreak

$ \vec{measX} = \vec{measY} \times \frac{\vec{p}}{|\vec{p}|} $
\pagebreak

$ d_{0} $
\pagebreak

$ \vec{d} $
\pagebreak

$ \vec{measX} $
\pagebreak

$ sign = -sign(\vec{d} \cdot \vec{measX}) $
\pagebreak

$ \vec l_{a}(\lambda) = \vec m_a + \lambda \cdot \vec e_{a} $
\pagebreak

$ \vec l_{b}(\mu) = \vec m_b + \mu \cdot \vec e_{b} $
\pagebreak

$ \vec s(\lambda, \mu) = \vec l_{b} - l_{a} = \vec m_{ab} + \mu \cdot \vec e_{b} - \lambda \cdot \vec e_{a} $
\pagebreak

$ \vec m_{ab} = \vec m_{b} - \vec m_{a} $
\pagebreak

$ \vec s(u, \mu_0) $
\pagebreak

$ \vec l_{a,0} = l_{a}(u) $
\pagebreak

$ \vec l_{b,0} = l_{b}(\mu_0) $
\pagebreak

$ \vec e_{a} $
\pagebreak

$ \vec e_{b} $
\pagebreak

$ 0 = \vec s(u, \mu_0) \cdot \vec e_a = \vec m_ab \cdot \vec e_a + \mu_0 \vec e_a \cdot \vec e_b - u $
\pagebreak

$ 0 = \vec s(u, \mu_0) \cdot \vec e_b = \vec m_ab \cdot \vec e_b + \mu_0 - u \vec e_b \cdot \vec e_a $
\pagebreak

$ u $
\pagebreak

$ \mu_0 $
\pagebreak

$ u = \frac{(\vec m_ab \cdot \vec e_a)-(\vec m_ab \cdot \vec e_b)(\vec e_a \cdot \vec e_b)}{1-(\vec e_a \cdot \vec e_b)^2} $
\pagebreak

$ \mu_0 = - \frac{(\vec m_ab \cdot \vec e_b)-(\vec m_ab \cdot \vec e_a)(\vec e_a \cdot \vec e_b)}{1-(\vec e_a \cdot \vec e_b)^2} $
\pagebreak

$ \vec n \cdot \vec x = \vec n \cdot \vec p,$
\pagebreak

$ \vec n = (n_{x}, n_{y}, n_{z})$
\pagebreak

$ \vec p = (p_{x}, p_{y}, p_{z})$
\pagebreak

$ \vec x = (x,y,z) $
\pagebreak

$ \vec l(u) = \vec l_{1} + u \cdot \vec v $
\pagebreak

$ u = \frac{\vec n (\vec p - \vec l_{1})}{\vec n \vec v}$
\pagebreak

$ eta $
\pagebreak

$ |x_{min}| $
\pagebreak

$ | x_{max} | $
\pagebreak

$ | y_{H} | $
\pagebreak

$ y = \kappa_{I} x + \delta_{I} $
\pagebreak

$ y = \kappa_{II} x + \delta_{II} $
\pagebreak

$ \kappa_{I} = - \kappa_{II} = 2 \frac{y_{H}}{x_{max} - x_{min}} $
\pagebreak

$ \delta_{I} = \delta_{II} = - \frac{1}{2}\kappa_{I}(x_{max} + x_{min}) $
\pagebreak

$[\text{xmin},\text{xmax})$
\pagebreak

$\text{nBins}$
\pagebreak

$l <= x < u$
\pagebreak

$1 \le \text{bin} \le \text{nBins} + 1$
\pagebreak

$0 \le \text{bin} \le \text{nBins}$
\pagebreak

$1 \le \text{bin} \le \text{nBins}$
\pagebreak

$\text{xmin} \le x < \text{xmax}$
\pagebreak

$\text{xmin_i} \le x_i < \text{xmax}_i \forall i=0, \dots, d-1$
\pagebreak

$2 \times \text{size}+1$
\pagebreak

$2^d$
\pagebreak

$d$
\pagebreak

$2^d = N $
\pagebreak

$ \alpha x^{2} + \beta x + \gamma = 0 $
\pagebreak

$ x_{1, 2} = - \frac{\beta \pm \sqrt{\beta^{2}-4\alpha\gamma}}{2\alpha}$
\pagebreak

$ \beta > 0 $
\pagebreak

$ x_{1} = - \frac{\beta + \sqrt{\beta^{2}-4\alpha\gamma}}{2\alpha} := \frac{q}{\alpha}$
\pagebreak

$ q= -\frac{1}{2}(\beta+sqrt{\beta^{2}-4\alpha\gamma})$
\pagebreak

$ x_{2} $
\pagebreak

$ x_{2} = \frac{\gamma}{q} = -\frac{2\gamma}{\beta+sqrt{\beta^{2}-4\alpha\gamma}}$
\pagebreak

$ -\frac{2\gamma}{\beta+sqrt{\beta^{2}-4\alpha\gamma}} = -\frac{2\gamma}{\beta}\frac{1}{1+\sqrt{1-4\alpha\gamma/\beta^{2}}}$
\pagebreak

$ x_{2}\frac{1}{1-\sqrt{1-4\alpha\gamma/\beta^{2}}} = -\frac{2\gamma}{\beta}\frac{1}{1-1+4\alpha\gamma/\beta^{2}}=-\frac{\beta}{2\alpha}.$
\pagebreak

$ -\frac{\beta(1-\sqrt{1-4\alpha\gamma/\beta^{2}}}{2\alpha} = - \frac{\beta - \sqrt{\beta^{2}-4\alpha\gamma}}{2\alpha} $
\pagebreak

$\text{lowerCorner}[i] \le \text{position}[i] \le \text{upperCorner}[i] \quad \forall i=0, \dots, d-1$
\pagebreak

$[-2^{53}+1, 2^{53}-1]$
\pagebreak

$ \ln(Z) $
\pagebreak

$ \ln(Z)/3 + f_c $
\pagebreak

$ ((Fel-fc)+Finel*invZ)$
\pagebreak

$ (Fel-fc)$
\pagebreak

$ (1.0+invZ)/12 $
\pagebreak

$E_\mathrm{sp}-E_\mathrm{i,A}$
\pagebreak

$E_\mathrm{sp}$
\pagebreak

$E_\mathrm{i,A}$
\pagebreak

$A$
\pagebreak

$b$
\pagebreak

\[ r(\theta) = \frac{(1-e^2)r_0/2}{1-e \sin(\theta-\theta_R/2)}, \]
\pagebreak

$e$
\pagebreak

\[ e = \sqrt{1+4b^2/r_0^2}; \]
\pagebreak

$\theta_R$
\pagebreak

\[ \theta_R = \pi - 2\arctan\left(\frac{2b}{r_0}\right) \]
\pagebreak

$\theta$
\pagebreak

$\pi$
\pagebreak

$r_0$
\pagebreak

\[ p_{CM}^2 = \frac{z^2 - m_1^2 m_2^2}{2 z + m_1^2 + m_2^2} \]
\pagebreak

\[ z = E_1 E_2 - \vec{p}_1\cdot\vec{p}_2 \]
\pagebreak

\[ p_{lab}^2 = \frac{s^2 - 2 s (m_1^2 + m_2^2) + {(m_1^2 - m_2^2)}^2}{4 m_2^2} \]
\pagebreak

\[ {\left(2.38\cdot\frac{9\pi}{2}\right)}^{1/6}\sqrt\hbar \]
\pagebreak

$2.38h$
\pagebreak

\[ \exp(B\cdot t) \]
\pagebreak

$B$
\pagebreak

$\exp(Bt)$
\pagebreak

\[ (0, \Delta\vec{x}), \]
\pagebreak

$\Delta\vec{x}$
\pagebreak

\[ (\Delta t', \Delta\vec{x}'), \]
\pagebreak

\[ |\Delta\vec{x}'| \leq \sqrt{\sigma/\pi}.\]
\pagebreak

$|\Delta\vec{x}'|\leq|\Delta\vec{x}|$
\pagebreak

$\exp(B\cdot t)$
\pagebreak

$\hbar$
\pagebreak

$\hbar c$
\pagebreak

$\hbar^2 c^2$
\pagebreak

\[ e^2/(4 pi epsilon_0) \]
\pagebreak

$\int_{x_0}^{x_1} f(x) dx$
\pagebreak

\[ m = \sqrt{E^2 - {\vec p}^2}\]
\pagebreak

\[ (A_1,Z_1) + (A_2, Z_2) --> (A_1+A_2,Z_1+Z_2) \]
\pagebreak

\[ (A_1,Z_1) + (A_2, Z_2) --> (A_3,Z_3) + (A1+A2-A3,Z1+Z2-Z3) \]
\pagebreak

\[ p_F(A)=\alpha-\beta\cdot e^{(-A\cdot\gamma)} \]
\pagebreak

$\alpha=259.416$
\pagebreak

$c$
\pagebreak

$\beta=152.824$
\pagebreak

$\gamma=9.5157\cdot10^{-2}$
\pagebreak

\[ L = \frac{[K + (K^2 - 1)^\frac{1}{2}]}{a} \]
\pagebreak

\[ K = 1 + \frac{b}{8a} \]
\pagebreak

\[ M = a*L-1 \]
\pagebreak

\end{document}
